<?xml version="1.0" encoding="UTF-8"?>
<rdf:RDF xmlns:rdf="http://www.w3.org/1999/02/22-rdf-syntax-ns#" xmlns:rdfs="http://www.w3.org/2000/01/rdf-schema#" xmlns:owl="http://www.w3.org/2002/07/owl#" xmlns:dcterms="http://purl.org/dc/terms/" xmlns:rddl="http://www.rddl.org/">
  <owl:Ontology rdf:about="http://open-services.net/ns/qm#">
    <dcterms:title>The OSLC Quality Management(QM) Vocabulary</dcterms:title>
    <dcterms:description rdf:parseType="Literal">
      All vocabulary URIs defined in the OSLC Quality Management (QM) namespace.
    </dcterms:description>
    <rdfs:label>Quality Management(QM)</rdfs:label>
    <rdfs:seeAlso rdf:resource="http://open-services.net/bin/view/Main/QmHome"/>
    <rdfs:seeAlso rdf:resource="http://open-services.net/bin/view/Main/QmSpecificationV2"/>
    <rdfs:seeAlso rdf:resource="http://open-services.net/ns/qm/qm.rdf"/>
    <rdfs:seeAlso>
      <rdf:Description rdf:about="http://open-services.net/ns/qm/qm.rdf">
        <rddl:nature rdf:resource="http://www.w3.org/2000/01/rdf-schema#"/>
      </rdf:Description>
    </rdfs:seeAlso>
  </owl:Ontology>
  <rdfs:Class rdf:about="http://open-services.net/ns/qm#TestPlan">
    <rdfs:isDefinedBy rdf:resource="http://open-services.net/ns/qm#"/>
    <rdfs:label>TestPlan</rdfs:label>
    <rdfs:comment>The QM Test Plan resource</rdfs:comment>
    <rdfs:seeAlso rdf:resource="http://open-services.net/bin/view/Main/QmSpecificationV2#Resource_TestPlan"/>
  </rdfs:Class>
  <rdfs:Class rdf:about="http://open-services.net/ns/qm#TestCase">
    <rdfs:isDefinedBy rdf:resource="http://open-services.net/ns/qm#"/>
    <rdfs:label>TestCase</rdfs:label>
    <rdfs:comment>The QM Test Case resource</rdfs:comment>
    <rdfs:seeAlso rdf:resource="http://open-services.net/bin/view/Main/QmSpecificationV2#Resource_TestCase"/>
  </rdfs:Class>
  <rdfs:Class rdf:about="http://open-services.net/ns/qm#TestScript">
    <rdfs:isDefinedBy rdf:resource="http://open-services.net/ns/qm#"/>
    <rdfs:label>TestScript</rdfs:label>
    <rdfs:comment>The QM Test Script resource</rdfs:comment>
    <rdfs:seeAlso rdf:resource="http://open-services.net/bin/view/Main/QmSpecificationV2#Resource_TestScript"/>
  </rdfs:Class>
  <rdfs:Class rdf:about="http://open-services.net/ns/qm#TestExecutionRecord">
    <rdfs:isDefinedBy rdf:resource="http://open-services.net/ns/qm#"/>
    <rdfs:label>TestExecutionRecord</rdfs:label>
    <rdfs:comment>The QM Test Execution Record resource</rdfs:comment>
    <rdfs:seeAlso rdf:resource="http://open-services.net/bin/view/Main/QmSpecificationV2#Resource_TestExecutionRecord"/>
  </rdfs:Class>
  <rdfs:Class rdf:about="http://open-services.net/ns/qm#TestResult">
    <rdfs:isDefinedBy rdf:resource="http://open-services.net/ns/qm#"/>
    <rdfs:label>TestResult</rdfs:label>
    <rdfs:comment>The QM Test Result resource</rdfs:comment>
    <rdfs:seeAlso rdf:resource="http://open-services.net/bin/view/Main/QmSpecificationV2#Resource_TestResult"/>
  </rdfs:Class>
  <rdf:Property rdf:about="http://open-services.net/ns/qm#relatedChangeRequest">
    <rdfs:isDefinedBy rdf:resource="http://open-services.net/ns/qm#"/>
    <rdfs:label>relatedChangeRequest</rdfs:label>
    <rdfs:comment>A related change request. It is likely that the target resource will be an oslc_cm:ChangeRequest but that is not necessarily the case. </rdfs:comment>
    <rdfs:range rdf:resource="http://open-services.net/ns/qm#TestPlan"/>
    <rdfs:range rdf:resource="http://open-services.net/ns/qm#TestCase"/>
    <rdfs:range rdf:resource="http://open-services.net/ns/qm#TestScript"/>
    <rdfs:range rdf:resource="http://open-services.net/ns/qm#TestExecutionRecord"/>
    <rdfs:range rdf:resource="http://open-services.net/ns/qm#TestResult"/>
    <rdfs:seeAlso rdf:resource="http://open-services.net/bin/view/Main/QmSpecificationV2#Resource_TestPlan"/>
    <rdfs:seeAlso rdf:resource="http://open-services.net/bin/view/Main/QmSpecificationV2#Resource_TestCase"/>
    <rdfs:seeAlso rdf:resource="http://open-services.net/bin/view/Main/QmSpecificationV2#Resource_TestScript"/>
    <rdfs:seeAlso rdf:resource="http://open-services.net/bin/view/Main/QmSpecificationV2#Resource_TestExecutionRecord"/>
    <rdfs:seeAlso rdf:resource="http://open-services.net/bin/view/Main/QmSpecificationV2#Resource_TestResult"/>
  </rdf:Property>
  <rdf:Property rdf:about="http://open-services.net/ns/qm#usesTestCase">
    <rdfs:isDefinedBy rdf:resource="http://open-services.net/ns/qm#"/>
    <rdfs:label>usesTestCase</rdfs:label>
    <rdfs:comment>Test Case used by the Test Plan. It is likely that the target resource will be an oslc_qm:TestCase but that is not necessarily the case.</rdfs:comment>
    <rdfs:range rdf:resource="http://open-services.net/ns/qm#TestPlan"/>
    <rdfs:seeAlso rdf:resource="http://open-services.net/bin/view/Main/QmSpecificationV2#Resource_TestPlan"/>
  </rdf:Property>
  <rdf:Property rdf:about="http://open-services.net/ns/qm#validatesRequirementCollection">
    <rdfs:isDefinedBy rdf:resource="http://open-services.net/ns/qm#"/>
    <rdfs:label>validatesRequirementCollection</rdfs:label>
    <rdfs:comment>Requirement Collection that is validated by the Test Plan. It is likely that the target resource will be an oslc_rm:RequirementCollection but that is not necessarily the case.</rdfs:comment>
    <rdfs:range rdf:resource="http://open-services.net/ns/qm#TestPlan"/>
    <rdfs:seeAlso rdf:resource="http://open-services.net/bin/view/Main/QmSpecificationV2#Resource_TestPlan"/>
  </rdf:Property>
  <rdf:Property rdf:about="http://open-services.net/ns/qm#testsChangeRequest">
    <rdfs:isDefinedBy rdf:resource="http://open-services.net/ns/qm#"/>
    <rdfs:label>testsChangeRequest</rdfs:label>
    <rdfs:comment>Change Request tested by the Test Case. It is likely that the target resource will be an oslc_cm:ChangeRequest but that is not necessarily the case.</rdfs:comment>
    <rdfs:range rdf:resource="http://open-services.net/ns/qm#TestCase"/>
    <rdfs:seeAlso rdf:resource="http://open-services.net/bin/view/Main/QmSpecificationV2#Resource_TestCase"/>
  </rdf:Property>
  <rdf:Property rdf:about="http://open-services.net/ns/qm#usesTestScript">
    <rdfs:isDefinedBy rdf:resource="http://open-services.net/ns/qm#"/>
    <rdfs:label>usesTestScript</rdfs:label>
    <rdfs:comment>Test Script used by the Test Case. It is likely that the target resource will be an oslc_qm:TestScript but that is not necessarily the case.</rdfs:comment>
    <rdfs:range rdf:resource="http://open-services.net/ns/qm#TestCase"/>
    <rdfs:seeAlso rdf:resource="http://open-services.net/bin/view/Main/QmSpecificationV2#Resource_TestCase"/>
  </rdf:Property>
  <rdf:Property rdf:about="http://open-services.net/ns/qm#validatesRequirement">
    <rdfs:isDefinedBy rdf:resource="http://open-services.net/ns/qm#"/>
    <rdfs:label>validatesRequirement</rdfs:label>
    <rdfs:comment>Requirement that is validated by the Test Case. It is likely that the target resource will be an oslc_rm:Requirement but that is not necessarily the case.</rdfs:comment>
    <rdfs:range rdf:resource="http://open-services.net/ns/qm#TestCase"/>
    <rdfs:range rdf:resource="http://open-services.net/ns/qm#TestScript"/>
    <rdfs:seeAlso rdf:resource="http://open-services.net/bin/view/Main/QmSpecificationV2#Resource_TestCase"/>
    <rdfs:seeAlso rdf:resource="http://open-services.net/bin/view/Main/QmSpecificationV2#Resource_TestScript"/>
  </rdf:Property>
  <rdf:Property rdf:about="http://open-services.net/ns/qm#executionInstructions">
    <rdfs:isDefinedBy rdf:resource="http://open-services.net/ns/qm#"/>
    <rdfs:label>executionInstructions</rdfs:label>
    <rdfs:comment>Instructions for executing the test script. Note that the value of Occurs is undefined. The resource shape document provided by the QM service provider may be consulted for its value.</rdfs:comment> 
    <rdfs:range rdf:resource="http://open-services.net/ns/qm#TestScript"/>
    <rdfs:seeAlso rdf:resource="http://open-services.net/bin/view/Main/QmSpecificationV2#Resource_TestScript"/>
  </rdf:Property>
  <rdf:Property rdf:about="http://open-services.net/ns/qm#blockedByChangeRequest">
    <rdfs:isDefinedBy rdf:resource="http://open-services.net/ns/qm#"/>
    <rdfs:label>blockedByChangeRequest</rdfs:label>
    <rdfs:comment>Change Request that prevents execution of the Test Execution Record. It is likely that the target resource will be an oslc_cm:ChangeRequest but that is not necessarily the case.</rdfs:comment>
    <rdfs:range rdf:resource="http://open-services.net/ns/qm#TestExecutionRecord"/>
    <rdfs:seeAlso rdf:resource="http://open-services.net/bin/view/Main/QmSpecificationV2#Resource_TestExecutionRecord"/>
  </rdf:Property>
  <rdf:Property rdf:about="http://open-services.net/ns/qm#runsOnTestEnvironment">
    <rdfs:isDefinedBy rdf:resource="http://open-services.net/ns/qm#"/>
    <rdfs:label>runsOnTestEnvironment</rdfs:label>
    <rdfs:comment>Indicates the environment details of the test case for this execution record.</rdfs:comment>
    <rdfs:range rdf:resource="http://open-services.net/ns/qm#TestExecutionRecord"/>
    <rdfs:seeAlso rdf:resource="http://open-services.net/bin/view/Main/QmSpecificationV2#Resource_TestExecutionRecord"/>
  </rdf:Property>
  <rdf:Property rdf:about="http://open-services.net/ns/qm#reportsOnTestPlan">
    <rdfs:isDefinedBy rdf:resource="http://open-services.net/ns/qm#"/>
    <rdfs:label>reportsOnTestPlan</rdfs:label>
    <rdfs:comment>Test Plan that the Test Execution Record reports on. It is likely that the target resource will be an oslc_qm:TestPlan but that is not necessarily the case.</rdfs:comment>
    <rdfs:range rdf:resource="http://open-services.net/ns/qm#TestExecutionRecord"/>
    <rdfs:seeAlso rdf:resource="http://open-services.net/bin/view/Main/QmSpecificationV2#Resource_TestExecutionRecord"/>
  </rdf:Property>
  <rdf:Property rdf:about="http://open-services.net/ns/qm#runsTestCase">
    <rdfs:isDefinedBy rdf:resource="http://open-services.net/ns/qm#"/>
    <rdfs:label>runsTestCase</rdfs:label>
    <rdfs:comment>Test Case run by the Test Execution Record. It is likely that the target resource will be an oslc_qm:TestCase but that is not necessarily the case.</rdfs:comment>
    <rdfs:range rdf:resource="http://open-services.net/ns/qm#TestExecutionRecord"/>
    <rdfs:seeAlso rdf:resource="http://open-services.net/bin/view/Main/QmSpecificationV2#Resource_TestExecutionRecord"/>
  </rdf:Property>
  <rdf:Property rdf:about="http://open-services.net/ns/qm#affectedByChangeRequest">
    <rdfs:isDefinedBy rdf:resource="http://open-services.net/ns/qm#"/>
    <rdfs:label>affectedByChangeRequest</rdfs:label>
    <rdfs:comment>Change request that affects the Test Result. It is likely that the target resource will be an oslc_cm:ChangeRequest but that is not necessarily the case.</rdfs:comment>
    <rdfs:range rdf:resource="http://open-services.net/ns/qm#TestResult"/>
    <rdfs:seeAlso rdf:resource="http://open-services.net/bin/view/Main/QmSpecificationV2#Resource_TestResult"/>
  </rdf:Property>
  <rdf:Property rdf:about="http://open-services.net/ns/qm#executesTestScript">
    <rdfs:isDefinedBy rdf:resource="http://open-services.net/ns/qm#"/>
    <rdfs:label>executesTestScript</rdfs:label>
    <rdfs:comment>Test Script executed to produce the Test Result. It is likely that the target resource will be an oslc_qm:TestScript but that is not necessarily the case.</rdfs:comment>
    <rdfs:range rdf:resource="http://open-services.net/ns/qm#TestResult"/>
    <rdfs:seeAlso rdf:resource="http://open-services.net/bin/view/Main/QmSpecificationV2#Resource_TestResult"/>
  </rdf:Property>
  <rdf:Property rdf:about="http://open-services.net/ns/qm#producedByTestExecutionRecord">
    <rdfs:isDefinedBy rdf:resource="http://open-services.net/ns/qm#"/>
    <rdfs:label>producedByTestExecutionRecord</rdfs:label>
    <rdfs:comment>Test Execution Record that the Test Result was produced by. It is likely that the target resource will be an oslc_qm:TestExecutionRecord but that is not necessarily the case.</rdfs:comment>
    <rdfs:range rdf:resource="http://open-services.net/ns/qm#TestResult"/>
    <rdfs:seeAlso rdf:resource="http://open-services.net/bin/view/Main/QmSpecificationV2#Resource_TestResult"/>
  </rdf:Property>
  <rdf:Property rdf:about="http://open-services.net/ns/qm#reportsOnTestCase">
    <rdfs:isDefinedBy rdf:resource="http://open-services.net/ns/qm#"/>
    <rdfs:label>reportsOnTestCase</rdfs:label>
    <rdfs:comment>Test Case that the Test Result reports on. It is likely that the target resource will be an oslc_qm:TestCase but that is not necessarily the case.</rdfs:comment>
    <rdfs:range rdf:resource="http://open-services.net/ns/qm#TestResult"/>
    <rdfs:seeAlso rdf:resource="http://open-services.net/bin/view/Main/QmSpecificationV2#Resource_TestResult"/>
  </rdf:Property>
  <rdf:Property rdf:about="http://open-services.net/ns/qm#reportsOnTestPlan">
    <rdfs:isDefinedBy rdf:resource="http://open-services.net/ns/qm#"/>
    <rdfs:label>reportsOnTestPlan</rdfs:label>
    <rdfs:comment>Test Plan that the Test Result reports on. It is likely that the target resource will be an oslc_qm:TestPlan but that is not necessarily the case.</rdfs:comment>
    <rdfs:range rdf:resource="http://open-services.net/ns/qm#TestResult"/>
    <rdfs:seeAlso rdf:resource="http://open-services.net/bin/view/Main/QmSpecificationV2#Resource_TestResult"/>
  </rdf:Property>
</rdf:RDF>
